Source/DafnyCore/Verifier/AlcorEngineTest.dfy
@@ -5,42 +5,84 @@ module AlcorEngineTest {
 
   method {:test} DummyProofFinderTest() {
     print "\n";
+    var ia := Identifier("a");
+    var ib := Identifier("b");
+    var ic := Identifier("c");
+    var id := Identifier("d");
+    var a := Var(ia);
+    var b := Var(ib);
+    var c := Var(ic);
+    var d := Var(id);
+    var remaining := Var(Identifier("remaining"));
     
-    var goal := Imp(And(And(Var("a"), Var("b")), Var("...")), Var("a"));
+    var goal := Imp(And(And(a, b), remaining), a);
     var expr :- expect DummyProofFinder(goal);
     print "Automatically found a proof of " + goal.ToString() + "\n";
 
-    goal := Imp(And(And(Var("a"), Var("b")), Var("...")), Var("b"));
+    goal := Imp(And(And(a, b), remaining), b);
     expr :- expect DummyProofFinder(goal);
     print "Automatically found a proof of " + goal.ToString() + "\n";
 
-    goal := Imp(And(Var("a"), And(Var("b"), And(Var("c"), And(Var("d"), Var("..."))))), Var("d"));
+    goal := Imp(And(a, And(b, And(c, And(d, remaining)))), d);
     expr :- expect DummyProofFinder(goal);
     print "Automatically found a proof of " + goal.ToString() + "\n";
 
     
-    goal := Imp(Var("..."), Imp(Var("b"), Var("b")));
+    goal := Imp(remaining, Imp(b, b));
     expr :- expect DummyProofFinder(goal);
     print "Automatically found a proof of " + goal.ToString() + "\n";
 
-    goal := Imp(Var("..."), Imp(And(Var("a"), Var("b")), Var("b")));
+    goal := Imp(remaining, Imp(And(a, b), b));
     expr :- expect DummyProofFinder(goal);
     print "Automatically found a proof of " + goal.ToString() + "\n";
 
-    goal := Imp(And(Imp(Var("a"), Var("b")), And(Var("a"), True)), Var("b"));
+    goal := Imp(And(Imp(a, b), And(a, True)), b);
     expr :- expect DummyProofFinder(goal);
     print "Automatically found a proof of " + goal.ToString() + "\n";
 
-    goal := Imp(And(Var("a"), And(Imp(Var("a"), Var("b")), True)), Var("b"));
+    goal := Imp(And(a, And(Imp(a, b), True)), b);
     expr :- expect DummyProofFinder(goal);
     print "Automatically found a proof of " + goal.ToString() + "\n";
 
-    goal := Imp(And(Var("a"), And(Var("b"), Var("..."))), And(Var("a"), Var("b")));
+    goal := Imp(And(a, And(b, remaining)), And(a, b));
     expr :- expect DummyProofFinder(goal);
     print "Automatically found a proof of " + goal.ToString() + "\n";
 
-    goal := Imp(And(Var("b"), And(Var("a"), Var("..."))), And(Var("a"), Var("b")));
+    goal := Imp(And(b, And(a, remaining)), And(a, b));
     expr :- expect DummyProofFinder(goal);
     print "Automatically found a proof of " + goal.ToString() + "\n";
   }
+
+  method {:test} ProofCheckerTest() {
+    print "\n";
+    var ia := Identifier("a");
+    var ib := Identifier("b");
+    var a := Var(ia);
+    var b := Var(ib);
+    
+    var goal := Forall(Abs(ia,
+                Forall(Abs(ib, Imp(And(Imp(a, b), a), And(b, a))))));
+
+    var proofProgram :=
+          ForallIntro.apply2(ProofExpr(a),
+            ForallIntro.apply2(ProofExpr(b),
+              ImpIntro.apply2(
+                ProofExpr(And(Imp(a, b), a)),
+                ProofAbs("env", Ind,
+                  Let("a", Ind, AndElimRight.apply1(ProofVar("env")),
+                  Let("aToB", Ind, AndElimLeft.apply1(ProofVar("env")),
+                  Let("b", Ind, ImpElim.apply2(ProofVar("aToB"), ProofVar("a")),
+                  AndIntro.apply2(ProofVar("b"), ProofVar("a")))))))));
+    var result :- expect CheckProof(proofProgram, EnvNil, goal);
+
+  }
 }
+
+
+
+
+
+
+
+
+
